%! TEX root = ./main.tex
\begin{exercise}[]{}
	Let $ f: \mathbb{R}^d \rightarrow (-\infty,+\infty] $ be even. Prove that $ f^{*} $ is even.
\end{exercise}

\begin{solution}[]
	We have for $ y\in \mathbb{R}^d $:
\begin{equation*}
	f^{*}(y) = \sup_{x\in \mathbb{R}^d} \siprod{y}{x} - f(x)
\end{equation*}
and 
\begin{align*}
	f^{*}(-y) &= \sup_{x \in \mathbb{R}^d} \siprod{-y}{x} - f(x) \\
		  &= \sup_{-x\in \mathbb{R}^d} \siprod{-y}{-x} - f(-x) \\
		  &= \sup_{x\in \mathbb{R}^d} \siprod{y}{x} - f(x) \\
		  &= f^{*}(y)
\end{align*}
Where we do the change of variable $ x \rightarrow -x $ in the second line and use the parity of $ f $ in the third line.
\end{solution}
