%! TEX root = ./main.tex
\begin{exercise}[]{}
	Prove the three-points equality for Bregman divergences in Lemma 6.6 :
\begin{equation*}
	\forall x,y \in \text{int} X, z \in X, \, B_{\psi}(z ; x) + B_{\psi}(x ; y) - B_{\psi}(z ; y) = \siprod{\nabla \psi(y)-\nabla \psi(x)}{z-x}
\end{equation*}

\end{exercise}

\begin{solution}[]
\begin{align*}
	&B_{\psi}(z ; x) + B_{\psi}(x ;y) - B_{\psi}(z ;y) \\
	=& \psi(z)-\psi(x) - \siprod{\nabla \psi(x)}{z-x} + \psi(x) - \psi(y) - \siprod{\nabla  \psi(y)}{x-y} -\psi(z) + \psi(y) + \siprod{\nabla \psi(y)}{z-y} \\
	=& -\siprod{\nabla \psi(x)}{z-x} + \siprod{\nabla \psi(y)}{y-x + z-y} \\
	=& \siprod{\nabla \psi(y) - \nabla \psi(x)}{z-x}
\end{align*}

\end{solution}
